+

src/Find_proof.thy
@@ -20,30 +20,147 @@ lemma wellformed_tree_children: "wellformed_tree x (Node(ks,rs)) \<longrightarro
   apply(force intro: FIXME)
   done
 
+lemma check_keys_eq_ck_ck: "
+check_keys l ks u = (check_keys l ks None & check_keys None ks u)
+"
+apply(simp add: check_keys_def)
+done
+
+
+declare  wellformed_context.simps[simp del]
+
+declare wellformed_context_def_2[simp del] (* not a simp? - may expand too far? or use anyway? *)
+
+declare ts_to_ms_def_2[simp] (* likely a simp *)
+declare dest_fts_state_t_def_2[simp] (* surely a simp *)
+
+lemma search_key_to_index: "
+(search_key_to_index ks k = i) \<longrightarrow> i : set(subtree_indexes (ks,rs))
+"
+apply(force intro:FIXME)
+done
+
+lemma subtree_indexes_trichotomy: " 
+i : set(subtree_indexes (ks,rs)) \<longrightarrow> 
+(min_child_index < i & i < max_child_index(ks,rs)) | 
+(i = min_child_index) | (i = max_child_index(ks,rs))"
+apply(force intro:FIXME)
+done
+
+(* the easy case *)
+lemma search_key_to_index_bound: "
+(search_key_to_index ks k = i) & 
+min_child_index < i &
+i < max_child_index(ks,rs) \<longrightarrow> (
+let (l,u) = get_lu_for_child ((ks,rs),i) in
+check_keys l [k] u)"
+apply(force intro: FIXME)
+done
+
+lemma lu_with_default_eq_lu: "
+min_child_index < i &
+i < max_child_index(ks,rs) \<longrightarrow>
+get_lu_for_child_with_parent_default x2 ((ks,rs),i) = get_lu_for_child ((ks,rs),i)"
+apply(force intro:FIXME)
+done
 
 (*
-lemma wellformed_context_cons: "wellformed_context (x#xs) = (wellformed_context_1 (x#xs) & wellformed_cnodewellformed_context xs)"
-  apply(simp)
-  done
+wellformed_fts_focus (ts_to_ms ts) (Node (ks, rs)) \<Longrightarrow>
+       wellformed_context ts \<Longrightarrow>
 *)
 
-(* FIXME move *)
-lemma keys_Cons: 
-"keys (Node (l, cs)) = l@((List.map keys cs) |> List.concat)"
-apply (simp add:keys_def rev_apply_def keys_1_def)
-apply (induct cs) apply (force simp add:keys_def rev_apply_def)+
+lemma get_parent_bounds_check_keys: "
+wellformed_fts_1 (Fts_state (k, Node (ks, rs), ts)) \<Longrightarrow>
+get_parent_bounds ts = (l1, u1) \<Longrightarrow>
+check_keys l1 [k] u1
+"
+apply(simp add: get_parent_bounds_def)
+apply(case_tac ts) apply(simp add: get_parent_bounds_def check_keys_def)
+apply(simp)
+apply(subgoal_tac "? n i x. a = Cnode(n,i,x)") prefer 2 apply(force intro:FIXME)
+apply(elim exE, simp)
+apply(simp add: wellformed_fts_1_def dest_cnode_t_def)
+apply(force simp add: check_keys_def)
 done
+
+definition main_property :: "fts_state_t \<Rightarrow> bool" where
+"main_property fts' = (
+  let (k,t,ts) = dest_fts_state_t fts' in
+  case ts of 
+  Nil \<Rightarrow> True
+  | cn#cns \<Rightarrow> (
+    let (n,i,x) = dest_cnode_t cn in
+    let (l,u) = x in
+    check_keys l [k] u
+  ))"
+
+lemma main_lemma: "(
+(* want to check_keys l [k] u *)
+total_order_key_lte --> (
+  wellformed_fts fts & (step_fts fts = Some fts') --> main_property fts'))
+"
+apply(simp add: main_property_def)
+apply(simp, intro allI impI, elim conjE)
+apply(subgoal_tac "? k t ts. fts = Fts_state(k,t,ts)") prefer 2 apply(force intro:FIXME)
+apply(elim exE, simp)
+apply(simp add: step_fts_def)
+apply(subgoal_tac "(? kvs. t = Leaf kvs) | (? ks rs. t = Node(ks,rs))") prefer 2 apply(force intro: FIXME)
+apply(erule disjE) apply(force)
+apply(elim exE, simp)
+apply(subgoal_tac "? i. search_key_to_index ks k = i") prefer 2 apply(force)
+apply(elim exE, simp)
+apply(drule_tac t=fts' in sym) apply(simp)
+apply(thin_tac "fts'=_")
+apply(simp add: dest_cnode_t_def)
+apply(subgoal_tac "
+   ? l0 u0. get_lu_for_child_with_parent_default (get_parent_bounds ts) ((ks, rs), i) = (l0,u0)") prefer 2 apply(force)
+apply(elim exE, simp)
+(* this is the goal we want *)
+apply(subgoal_tac "check_keys l0 [k] None & check_keys None [k] u0") apply(force intro:FIXME)
+apply(rule conjI)
+ (* want check_keys l0 [k] None; distinguish i=min_child from other case *)
+ apply(subgoal_tac "(i = min_child_index) | (min_child_index < i & i \<le> max_child_index(ks,rs))") prefer 2 apply(force intro:FIXME)
+ apply(elim disjE)
+  (* i = min_child_index; so l0 is the lower bound of the parent *)
+  apply(subgoal_tac "? l1 u1. get_parent_bounds ts = (l1,u1)") prefer 2 apply(force intro:FIXME)
+  apply(elim exE,simp)
+  apply(subgoal_tac "l0 = l1") prefer 2 apply(force intro:FIXME)
+  apply(simp)
+  apply(simp add: wellformed_fts_def ) apply(elim conjE)
+  using check_keys_eq_ck_ck get_parent_bounds_check_keys apply blast
+    
+  (* min_child_index < i *)
+  apply(force intro:FIXME)
+
+ (* want check_keys None [k] u0 *)
+  apply(subgoal_tac "? l1 u1. get_parent_bounds ts = (l1,u1)") prefer 2 apply(force intro:FIXME)
+  apply(elim exE,simp)
+  apply(subgoal_tac "u0 = u1") prefer 2 apply(force intro:FIXME)
+  apply(simp)
+  apply(simp add: wellformed_fts_def ) apply(elim conjE)
+  using check_keys_eq_ck_ck get_parent_bounds_check_keys apply blast
+done 
+
 
 (* intuitively, we examine all the possible cases... *)
 lemma invariant_wf_fts: "invariant_wf_fts"
 apply (simp add:invariant_wf_fts_def)
 apply(intro impI allI)
+apply(subgoal_tac "(step_fts fts = None) | (? fts'. step_fts fts = Some(Fts_state(fts')))")
+  prefer 2 apply(force intro:FIXME)
+apply(erule disjE) apply(force)
+apply(elim exE)
+apply(simp)
+apply(subgoal_tac "main_property (Fts_state(fts'))")
+ prefer 2 apply (simp add: main_lemma option.case_eq_if)
 apply(simp add: step_fts_def)
 apply(subgoal_tac "? k t ts. fts = Fts_state(k,t,ts)") prefer 2 apply(force intro: FIXME)
 apply(elim exE, simp)
-apply(simp add: dest_fts_state_t_def)
-apply(subgoal_tac "(? ks rs. t = Node(ks,rs)) | (? kvs. t = Leaf kvs)") prefer 2 apply(force intro:FIXME)
+apply(subgoal_tac "(? kvs. t = Leaf kvs) | (? ks rs. t = Node(ks,rs))") prefer 2 apply(force intro:FIXME)
 apply(erule disjE)
+ (* Leaf *)
+ apply(force)
+
  (* t = Node(ks,rs) *)
  apply(elim exE, simp)
  apply(subgoal_tac "? i. search_key_to_index ks k = i") prefer 2 apply(force)
@@ -60,7 +177,7 @@ apply(erule disjE)
  apply(subgoal_tac "? r. r : set(rs) &  (rs ! i) = r") prefer 2 apply(force intro:FIXME)
  apply(elim exE conjE, simp)
  apply(simp add: wellformed_fts_def)
- apply(simp add: dest_fts_state_t_def)
+ apply(drule_tac t=fts' in sym) apply(simp) apply(thin_tac "fts'=_")
  apply(elim conjE)
  apply(intro conjI)
   (* wellformed_fts_focus rs!x since wf_fts_1 Node(_,rs) *)
@@ -68,31 +185,25 @@ apply(erule disjE)
   (* since Node(ks,rs) is wellformed, so too is rs!i *)
   apply(subgoal_tac "? ms. wellformed_tree ms (Node(ks,rs))") prefer 2 apply(force)
   apply(elim exE)
-  using wellformed_tree_children apply blast
+  using wellformed_tree_children apply( blast)
 
-  (* want wellformed_cnode *)
+  (* want wellformed_cnode Cnode(ks,rs,i,l0,u0) *)
+  apply(simp add: wellformed_context_def_2)
   apply(simp add: wellformed_cnode_def dest_cnode_t_def)
   apply(rule conjI)
    (* want wellformed_tree *)
-   apply(subgoal_tac "ts = Nil | (? cn2 rest. ts = cn2#rest)") prefer 2 apply(force intro: FIXME)
-   apply(elim disjE)
-    apply(simp)
-    apply(force simp add: wellformed_fts_focus_def)
-
-    apply(elim exE, simp)
-    apply(force simp add: wellformed_fts_focus_def)
+   apply(force simp add: wellformed_fts_focus_def)
 
    (* check_keys l0 (keys r) u0 ; suppose pb is a bound for rs, then lget_lu_with_def is a bound for rs!i *)
-    apply(force intro: FIXME)
+   apply(force intro: FIXME)
 
   (* want wellformed_fts_1 k,r,cn1#ts *)
-  apply(simp add: wellformed_fts_1_def dest_fts_state_t_def dest_cnode_t_def)
-  (* want check_keys l0 [k] u0 - this comes from the fact that k is the search key, and this is bounded *)
+  apply(simp (no_asm) add: wellformed_fts_1_def dest_fts_state_t_def dest_cnode_t_def)
+  apply(simp)
+  (* want check_keys l0 [k] u0 this comes from the fact that k is the search key, and this is bounded *)
   (* FIXME need lemma about get_lu_for_child *)
-  apply(force intro: FIXME)
+  apply(force simp add: main_property_def dest_cnode_t_def)
 
- (* Leaf *)
- apply(force)
 done
 
 end
