src/Tree_stack.thy
@@ -1,8 +1,6 @@
 theory Tree_stack imports Tree begin
 
-datatype xtra_t = Xtra "(key option * key option)"  (* l,u *)
-definition dest_xtra_t :: "xtra_t \<Rightarrow> key option * key option" where
-"dest_xtra_t x = (case x of Xtra (l,u) \<Rightarrow> (l,u))"
+type_synonym xtra_t = "(key option * key option)"  (* l,u *)
 
 datatype cnode_t = Cnode "node_t * nat * xtra_t"  (* n,i,x *)
 definition dest_cnode_t :: "cnode_t \<Rightarrow> node_t * nat * xtra_t" where
@@ -18,21 +16,19 @@ type_synonym tree_stack_t = "cnode_t list"
 definition get_parent_bounds :: "context_t \<Rightarrow> xtra_t" where
 "get_parent_bounds ts = (
   case ts of 
-  Nil \<Rightarrow> Xtra(None,None)
+  Nil \<Rightarrow> (None,None)
   | cn#_ \<Rightarrow> (let (n,i,x) = dest_cnode_t cn in x))"
 
 
 (* version of get_lu if parent bound is known *)
-(* FIXME dest_xtra_t is a bit boring *)
 definition get_lu_for_child_with_parent_default :: "xtra_t \<Rightarrow> (node_t*nat) \<Rightarrow> xtra_t" where
 "get_lu_for_child_with_parent_default x2 ni = (
-  let x1 = Xtra(get_lu_for_child ni) in
-  let (l1,u1) = dest_xtra_t x1 in
-  let (l2,u2) = dest_xtra_t x2 in
+  let (l1,u1) = get_lu_for_child ni in
+  let (l2,u2) = x2 in
   let l = (case l1 = None of True \<Rightarrow> l2 | _ \<Rightarrow> l1) in
   let u = (case u1 = None of True \<Rightarrow> u2 | _ \<Rightarrow> u1) in
-  Xtra(l,u)
-)
+  (l,u)
+)"
 
 (* FIXME adjust scala defns *)      
 definition wellformed_cnode :: "ms_t => xtra_t \<Rightarrow> cnode_t => bool " where
@@ -41,25 +37,39 @@ definition wellformed_cnode :: "ms_t => xtra_t \<Rightarrow> cnode_t => bool " w
   let (ks,rs) = n1 in
   let b1 = wellformed_tree ms (Node(ks,rs)) in  (* FIXME wellformed_kv_tree *)
   let b2 = i1 : set(subtree_indexes (ks,rs)) in
-  let (l1,u1) = dest_xtra_t x1 in
+  let (l1,u1) = x1 in
   let b3 = check_keys l1 (keys (rs!i1)) u1 in
-  let (l2,u2) = dest_xtra_t x2 in
-  let b4 = (case (i1 = min_child_index) of True \<Rightarrow> (l1 = l2) | False \<Rightarrow> True) in
-  let b5 = (case (i1 = max_child_index(n1)) of True \<Rightarrow> (u1 = u2) | False \<Rightarrow> True) in
-  b1&b2&b3&b4&b5)
+  let b4 = (x1 = get_lu_for_child_with_parent_default x2 (n1,i1)) in
+  b1&b2&b3&b4)
 "
+
+definition ts_to_ms :: "tree_stack_t \<Rightarrow> ms_t" where
+"ts_to_ms ts = (case ts of Nil \<Rightarrow> (Some Small_root_node_or_leaf) | _ \<Rightarrow> None)"
+
+lemma ts_to_ms_def_2: "
+  (ts_to_ms Nil = (Some Small_root_node_or_leaf)) &
+  (! x xs. ts_to_ms (x#xs) = None)"
+  apply(simp add:ts_to_ms_def)
+  done
 
 fun wellformed_context :: "context_t => bool" where
 "wellformed_context xs = (
   case xs of Nil \<Rightarrow> True
   | cn#cns \<Rightarrow> (
-    let ms = (case cns of Nil \<Rightarrow> (Some(Small_root_node_or_leaf)) | _ \<Rightarrow> None) in
+    let ms = ts_to_ms cns in
     let x2 = get_parent_bounds cns in
     wellformed_cnode ms x2 cn & 
     wellformed_context cns))"
 (*end wfcontext definition*)
 
-
+lemma wellformed_context_def_2: "
+  (wellformed_context  Nil = True) &
+  (wellformed_context (cn#cns) = (   
+    let ms = ts_to_ms cns in
+    let x2 = get_parent_bounds cns in
+    wellformed_cnode ms x2 cn & 
+    wellformed_context cns))"
+by simp
 
 (* old ---------------------------------------- *)
 
